adding client hello and server hello flights to HSL receive

src/tls/HSL.Receive.fst
@@ -33,10 +33,14 @@ module E = FStar.Error
 
 module HSM13 = Parsers.Handshake13
 module HSM12 = Parsers.Handshake12
+module HSM   = Parsers.Handshake
+
 module HSMType = Parsers.HandshakeType
 module R = MITLS.Repr
+
 module HSM13R = MITLS.Repr.Handshake13
 module HSM12R = MITLS.Repr.Handshake12
+module HSMR   = MITLS.Repr.Handshake
 
 open HSL.Common
 
@@ -405,6 +409,16 @@ let parse_hsm12_fin
       HSMType.Finished
       HSM12.handshake12_accessor_finished
 
+let parse_hsm12_nst
+  =  parse_hsm12
+      HSMType.New_session_ticket
+      HSM12.handshake12_accessor_new_session_ticket
+
+let parse_hsm12_cke
+  =  parse_hsm12
+      HSMType.Client_key_exchange
+      HSM12.handshake12_accessor_client_key_exchange
+
 let receive_flight12_c_ske_shd st b from to =
   let r = parse_hsm12_c b from in
   match r with
@@ -473,3 +487,105 @@ let receive_flight12_fin st b from to =
       reset_incremental_state st;
       E.Correct (Some ({ fin_msg = fin_repr }))
     end
+
+let receive_flight12_nst st b from to =
+  let r = parse_hsm12_nst b from in
+  match r with
+  | E.Error _ | E.Correct None ->
+    err_or_insufficient_data r F12_nst st b from to
+  | E.Correct (Some (nst_repr, pos)) ->
+    if pos <> to then E.Error bytes_remain_error
+    else begin
+      reset_incremental_state st;
+      E.Correct (Some ({ nst_msg = nst_repr }))
+    end
+
+let receive_flight12_cke st b from to =
+  let r = parse_hsm12_cke b from in
+  match r with
+  | E.Error _ | E.Correct None ->
+    err_or_insufficient_data r F12_cke st b from to
+  | E.Correct (Some (cke_repr, pos)) ->
+    if pos <> to then E.Error bytes_remain_error
+    else begin
+      reset_incremental_state st;
+      E.Correct (Some ({ cke_msg = cke_repr }))
+    end
+
+
+inline_for_extraction
+noextract
+let parse_hsm
+  (#a:Type) (#k:R.strong_parser_kind)
+  (#p:LP.parser k a) (#cl:LP.clens HSM.handshake a)
+  (#gacc:LP.gaccessor HSM.handshake_parser p cl)
+  (tag:HSMType.handshakeType{
+    forall (m:HSM.handshake).
+      (HSM.tag_of_handshake m == tag) <==> cl.LP.clens_cond m})
+  (acc:LP.accessor gacc)
+  : b:R.slice -> from:uint_32 ->
+    Stack (TLSError.result (option (HSMR.repr b & uint_32)))
+    (requires fun h ->
+      B.live h b.LP.base /\
+      from <= b.LP.len)
+    (ensures fun h0 r h1 ->
+      B.modifies B.loc_none h0 h1 /\
+      (match r with
+       | E.Error _ -> True
+       | E.Correct None -> True
+       | E.Correct (Some (repr, pos)) ->
+         repr.R.start_pos == from /\
+         repr.R.end_pos == pos /\
+         R.valid repr h1 /\
+         cl.LP.clens_cond (R.value repr)))
+         
+  = fun b from ->
+    
+    let pos = HSM.handshake_validator b from in
+
+    if pos <= LP.validator_max_length then begin
+      let parsed_tag = HSMType.handshakeType_reader b from in
+      if parsed_tag = tag then
+        let r = R.mk b from pos HSM.handshake_parser in
+        E.Correct (Some (r, pos))
+      else E.Error unexpected_flight_error
+    end
+    else if pos = LP.validator_error_not_enough_data then E.Correct None
+    else E.Error parsing_error
+
+let parse_hsm_ch
+  =  parse_hsm
+      HSMType.Client_hello
+      HSM.handshake_accessor_client_hello
+
+let parse_hsm_sh
+  = parse_hsm
+      HSMType.Server_hello
+      HSM.handshake_accessor_server_hello
+
+
+let receive_flight_ch st b from to =
+  let r = parse_hsm_ch b from in
+  match r with
+  | E.Error _ | E.Correct None ->
+    err_or_insufficient_data r F_ch st b from to
+  | E.Correct (Some (ch_repr, pos)) ->
+    if pos <> to then E.Error bytes_remain_error
+    else begin
+      reset_incremental_state st;
+      E.Correct (Some ({ ch_msg = ch_repr }))
+    end
+
+let receive_flight_sh st b from to =
+  let r = parse_hsm_sh b from in
+  match r with
+  | E.Error _ | E.Correct None ->
+    err_or_insufficient_data r F_sh st b from to
+  | E.Correct (Some (sh_repr, pos)) ->
+    if pos <> to then E.Error bytes_remain_error
+    else begin
+      reset_incremental_state st;
+      E.Correct (Some ({ sh_msg = sh_repr }))
+    end
+
+
